Implement prove_sem_thm (to replace whole_prog_thm)

basis/basis_ffiLib.sig
@@ -9,4 +9,10 @@ signature basis_ffiLib = sig
 
   val whole_prog_thm : ml_progLib.ml_prog_state -> string -> thm -> thm * term
 
+  (* arguments to prove_sem_thm:
+      - name of main function
+      - name to use for code definition
+      - whole_prog_spec thm              *)
+  val prove_sem_thm : string -> string -> thm -> thm
+
 end
