basis/basis_ffiScript.sml
@@ -3,8 +3,8 @@
 *)
 Theory basis_ffi
 Ancestors
-  ml_translator set_sep fsFFI fsFFIProps CommandLineProof
-  TextIOProof runtimeFFI RuntimeProof
+  ml_translator set_sep clFFI fsFFI fsFFIProps CommandLineProof
+  TextIOProg TextIOProof runtimeFFI RuntimeProof
 Libs
   preamble ml_translatorLib ml_progLib cfLib basisFunctionsLib
 
@@ -747,3 +747,166 @@ Theorem same_eval_state:
 Proof
   fs [semanticPrimitivesTheory.state_component_equality]
 QED
+
+Theorem iobuff_loc_eq:
+  iobuff_loc = Loc T 1
+Proof
+  simp [TextIOProgTheory.iobuff_loc_def]
+  \\ simp (find "refs_def" |> map snd |> map (fn (x,_,_) => x))
+QED
+
+Definition is_refs_basis_def:
+  is_refs_basis refs =
+    ?bs1 bs2 rest.
+       refs = W8array bs1 :: W8array bs2 :: rest /\
+       2052 <= LENGTH bs2
+End
+
+Theorem SPLIT_eq_SUBSET[local]:
+  (∃h_i. h_i ⊆ s ∧ P h_i) ⇒
+  (∃h_i h_k. SPLIT s (h_i,h_k) ∧ P h_i)
+Proof
+  rw [] \\ pop_assum $ irule_at Any
+  \\ qexists ‘s DIFF h_i’
+  \\ fs [SPLIT_def,IN_DISJOINT,EXTENSION,SUBSET_DEF]
+  \\ metis_tac []
+QED
+
+Theorem del_del_eq_sing[local]:
+  h_i = {x1;x2;m} ∧ x1 ≠ m ∧ x2 ≠ m ⇒ h_i DELETE x1 DELETE x2 = {m}
+Proof
+  fs [EXTENSION] \\ metis_tac []
+QED
+
+Theorem IMP_STDIO[local]:
+  res_st.ffi = basis_ffi cl fs ∧ wfcl cl ∧ wfFS fs ∧ STD_streams fs ∧
+  is_refs_basis res_st.refs ⇒
+  ∃h_i h_k.
+    SPLIT (st2heap (basis_proj1,basis_proj2) res_st) (h_i,h_k) ∧
+    (COMMANDLINE cl * STDIO fs * &T) h_i
+Proof
+  fs[cfStoreTheory.st2heap_def, cfStoreTheory.FFI_part_NOT_IN_store2heap,
+     cfStoreTheory.Mem_NOT_IN_ffi2heap, cfStoreTheory.ffi2heap_def,
+     is_refs_basis_def]
+  \\ qmatch_goalsub_abbrev_tac`parts_ok ffii (basis_proj1,basis_proj2)`
+  \\ strip_tac
+  \\ `parts_ok ffii (basis_proj1,basis_proj2)` by
+    (fs[Abbr`ffii`]
+     \\ rw[cfStoreTheory.parts_ok_def]
+     >- EVAL_TAC
+     >- EVAL_TAC
+     >~ [‘_ |++ _’]
+     >- (imp_res_tac oracle_parts
+         \\ first_x_assum $ qspec_then ‘res_st’ mp_tac
+         \\ fs [basis_ffi_def])
+    \\ qpat_x_assum`MEM _ basis_proj2`mp_tac
+    \\ simp[basis_proj2_def,basis_ffi_part_defs,cfHeapsBaseTheory.mk_proj2_def]
+    \\ TRY (qpat_x_assum`_ = SOME _`mp_tac)
+    \\ simp[basis_proj1_def,basis_ffi_part_defs,cfHeapsBaseTheory.mk_proj1_def,FUPDATE_LIST_THM]
+    \\ rw[] \\ rw[] \\ pairarg_tac \\ fs[FLOOKUP_UPDATE] \\ rw[]
+    \\ fs [AllCaseEqs(), SF DNF_ss, basis_ffi_def]
+    \\ fs[FAPPLY_FUPDATE_THM,cfHeapsBaseTheory.mk_ffi_next_def]
+    \\ TRY PURE_FULL_CASE_TAC
+    \\ fs[]
+    \\ EVERY (map imp_res_tac (CONJUNCTS basis_ffi_length_thms))
+    \\ fs[fs_ffi_no_ffi_div,cl_ffi_no_ffi_div]
+    \\ srw_tac[DNF_ss][] \\ simp[basis_ffi_oracle_def])
+  \\ fs[Abbr`ffii`, SEP_CLAUSES]
+  \\ simp [cfStoreTheory.store2heap_def,cfStoreTheory.store2heap_aux_def]
+  \\ irule SPLIT_eq_SUBSET
+  \\ simp [COMMANDLINE_def, SEP_CLAUSES, IOx_def, cl_ffi_part_def, IO_def,
+           SEP_EXISTS_THM, one_STAR, PULL_EXISTS]
+  \\ simp [STDIO_def, SEP_CLAUSES, IOx_def, cl_ffi_part_def, IO_def, GSYM STAR_ASSOC,
+           SEP_EXISTS_THM, one_STAR, PULL_EXISTS, IOFS_def, fs_ffi_part_def, cond_STAR]
+  \\ simp [SEP_EXISTS_THM, IOFS_iobuff_def, cond_STAR, W8ARRAY_def, iobuff_loc_eq]
+  \\ simp [cell_def, one_def, PULL_EXISTS, GREATER_EQ]
+  \\ irule_at Any del_del_eq_sing
+  \\ gvs [cfStoreTheory.FFI_part_NOT_IN_store2heap_aux]
+  \\ gvs [SF DNF_ss, basis_proj1_def, basis_ffi_def,FLOOKUP_SIMP,
+          alistTheory.flookup_fupdate_list,APPEND,
+          runtimeFFITheory.runtime_ffi_part_def,
+          mk_proj1_def, cl_ffi_part_def, fs_ffi_part_def]
+  \\ gvs [basis_proj2_def, mk_proj2_def, cl_ffi_part_def, fs_ffi_part_def]
+  \\ gvs [IO_fs_component_equality]
+  \\ ‘((fs with numchars := fs.numchars)) = fs’
+    by fs [IO_fs_component_equality]
+  \\ asm_rewrite_tac []
+QED
+
+Theorem whole_prog_spec_IMP':
+  whole_prog_spec main_v cl fs NONE post ∧
+  Decls init_env (init_state (basis_ffi cl fs) with eval_state := es) decs res_env res_st
+  ⇒
+  ∀main_name.
+    let all_decs = SNOC (Dlet unknown_loc (Pcon NONE [])
+                     (App Opapp [Var (Short main_name); Con NONE []])) decs in
+    nsLookup res_env.v (Short main_name) = SOME main_v
+    ⇒
+    res_st.ffi = basis_ffi cl fs
+    ⇒
+    is_refs_basis res_st.refs
+    ⇒
+    wfcl cl ∧ wfFS fs ∧ STD_streams fs ⇒
+    ∃io_events result.
+      semantics_dec_list
+        (init_state (basis_ffi cl fs) with eval_state := es) init_env
+        all_decs
+        (Terminate Success io_events) ∧
+      extract_fs fs io_events = SOME result ∧
+      post result
+Proof
+  simp [] \\ rpt strip_tac
+  \\ irule whole_prog_spec_semantics_prog
+  \\ gvs [ml_progTheory.lookup_var_def]
+  \\ last_x_assum $ irule_at Any
+  \\ pop_assum $ assume_tac o GSYM \\ fs []
+  \\ last_x_assum $ irule_at Any \\ fs []
+  \\ drule_all IMP_STDIO \\ strip_tac
+  \\ pop_assum $ irule_at Any
+  \\ pop_assum $ irule_at Any
+QED
+
+Theorem whole_prog_spec_IMP:
+  whole_prog_spec main_v cl fs NONE post ∧
+  Decls init_env (init_state (basis_ffi cl fs)) decs res_env res_st
+  ⇒
+  ∀main_name.
+    let all_decs = SNOC (Dlet unknown_loc (Pcon NONE [])
+                     (App Opapp [Var (Short main_name); Con NONE []])) decs in
+    nsLookup res_env.v (Short main_name) = SOME main_v
+    ⇒
+    res_st.ffi = basis_ffi cl fs
+    ⇒
+    is_refs_basis res_st.refs
+    ⇒
+    wfcl cl ∧ wfFS fs ∧ STD_streams fs ⇒
+    ∃io_events result.
+      semantics_dec_list
+        (init_state (basis_ffi cl fs)) init_env
+        all_decs
+        (Terminate Success io_events) ∧
+      extract_fs fs io_events = SOME result ∧
+      post result
+Proof
+  simp [] \\ rpt strip_tac
+  \\ ‘init_state (basis_ffi cl fs) =
+      init_state (basis_ffi cl fs) with eval_state :=
+      (init_state (basis_ffi cl fs)).eval_state’ by
+    gvs [ml_progTheory.init_state_def]
+  \\ first_assum $ once_rewrite_tac o single
+  \\ irule whole_prog_spec_semantics_prog
+  \\ gvs [ml_progTheory.lookup_var_def]
+  \\ last_x_assum $ irule_at Any
+  \\ pop_assum $ assume_tac o GSYM \\ fs []
+  \\ last_x_assum $ irule_at Any \\ fs []
+  \\ drule_all IMP_STDIO \\ strip_tac
+  \\ pop_assum $ irule_at Any
+  \\ pop_assum $ irule_at Any
+QED
+
+val ref_eq_nil_pat = “_ = [] : v store_v list”
+Theorem basis_refs_eqs =
+  find "refs_def"
+    |> map (fn (_,(x,_,_)) => x)
+    |> filter (can (match_term ref_eq_nil_pat) o concl)
+    |> LIST_CONJ;
