basis/basis_ffiLib.sml
@@ -104,30 +104,26 @@ fun subset_basis_st st precond sets sets_thm =
     foldl (uncurry PROVE_HYP) th length_hyps
   end;
 
-val whole_prog_spec_tm' = prim_mk_const{Thy="basis_ffi",Name="whole_prog_spec"}
-val whole_prog_spec2_tm = prim_mk_const{Thy="basis_ffi",Name="whole_prog_spec2"}
-val whole_prog_ffidiv_spec_tm = prim_mk_const{Thy="basis_ffi",Name="whole_prog_ffidiv_spec"}
-
 fun whole_prog_thm st name spec =
   let
     val call_ERR = ERR "whole_prog_thm"
     val whole_prog_spec_tm = spec |> concl |> strip_imp |> snd |> strip_comb |> fst
     val (whole_prog_spec_thm,sets_term,sets_theorem) =
-        if same_const whole_prog_spec_tm whole_prog_spec_tm' orelse
-           same_const whole_prog_spec_tm whole_prog_spec2_tm
+        if same_const whole_prog_spec_tm ``whole_prog_spec`` orelse
+           same_const whole_prog_spec_tm ``whole_prog_spec2``
         then
           let
             val sets_thm = mk_user_sets_thm ()
             val sets     = rand (concl sets_thm)
             val thm =
-              if same_const whole_prog_spec_tm whole_prog_spec_tm' then
+              if same_const whole_prog_spec_tm ``whole_prog_spec`` then
                 whole_prog_spec_semantics_prog
               else
                 whole_prog_spec2_semantics_prog
           in
             (thm, sets, sets_thm)
           end
-        else if same_const whole_prog_spec_tm whole_prog_ffidiv_spec_tm then
+        else if same_const whole_prog_spec_tm ``whole_prog_ffidiv_spec`` then
           (whole_prog_spec_semantics_prog_ffidiv,sets2,sets_thm2)
        else raise(call_ERR "Conclusion must be a whole_prog_spec or whole_prog_spec2 or whole_prog_ffidiv_spec")
     val ffi_v = st |> get_Decls_thm |> concl |> free_vars
@@ -159,5 +155,75 @@ fun whole_prog_thm st name spec =
              |> REWRITE_RULE [GSYM AND_IMP_INTRO]
              |> UNDISCH_ALL
   in (th,rhs(concl prog_rewrite)) end;
+
+val basis_ffi_term =
+  basis_ffiTheory.whole_prog_spec_IMP
+  |> concl |> rator |> rand |> rand
+  |> rator |> rator |> rator |> rand |> rand;
+
+fun simple_timer t = let
+  val new_t = Time.now()
+  val _ = print (" " ^ Time.fmt 1 (new_t - t) ^ " seconds\n")
+  in new_t end;
+
+fun prove_sem_thm name code_const_name spec = let
+  val t = Time.now()
+  fun print_pad s =
+    print (s ^ " " ^ implode (List.tabulate(Int.max(0,50 - String.size s), K #"_")))
+  val _ = print_pad ("prove_sem_thm: collecting declarations")
+  val Decls_lemma =
+    ml_translatorLib.get_ml_prog_state ()
+    |> ml_progLib.get_thm
+    |> REWRITE_RULE [ml_progTheory.ML_code_def,ml_progTheory.ML_code_env_def]
+  val t = simple_timer t
+  val _ = print_pad ("prove_sem_thm: instantiating main theorem")
+  val spec = spec |> UNDISCH_ALL
+  val th1 = CONJ spec (Decls_lemma |> GEN_ALL |> ISPEC basis_ffi_term |> SPEC_ALL);
+  val th2 = (MATCH_MP basis_ffiTheory.whole_prog_spec_IMP th1
+             handle HOL_ERR _ =>
+             MATCH_MP basis_ffiTheory.whole_prog_spec_IMP' th1)
+  val t = simple_timer t
+  val _ = print_pad ("prove_sem_thm: removing snocs from code")
+  val remove_snocs_conv =
+        PURE_REWRITE_CONV [listTheory.SNOC_APPEND] THENC
+        PURE_REWRITE_CONV [GSYM listTheory.APPEND_ASSOC] THENC
+        PURE_REWRITE_CONV [listTheory.APPEND]
+  val th3 = SPEC (mlstringSyntax.mk_mlstring name) th2
+            |> CONV_RULE (RAND_CONV remove_snocs_conv)
+  val code_tm = th3 |> concl |> rand
+  val code_v = mk_var(code_const_name, type_of code_tm)
+  val t = simple_timer t
+  val _ = print_pad ("prove_sem_thm: defining " ^ code_const_name)
+  val code_def = new_definition(code_const_name ^ "_def[compute]",mk_eq(code_v,code_tm))
+  val th4 = th3 |> CONV_RULE (RAND_CONV (K (SYM code_def)))
+                |> CONV_RULE (REWR_CONV LET_THM THENC BETA_CONV)
+  val t = simple_timer t
+  val _ = print_pad ("prove_sem_thm: using nsLookup for " ^ name ^ " in env")
+  val th5 = let
+    val g1 = th4 |> concl |> dest_imp |> fst
+    val l = dest_eq g1 |> fst |> nsLookup_conv
+    val l1 = prove(g1,REWRITE_TAC [l])
+    in MP th4 l1 end
+  val t = simple_timer t
+  val _ = print_pad ("prove_sem_thm: proving ffi is unchanged")
+  val th6 = let
+    val g2 = th5 |> concl |> dest_imp |> fst
+    val l2 = prove(g2,EVAL_TAC)
+    in MP th5 l2 end
+  val t = simple_timer t
+  val _ = print_pad ("prove_sem_thm: checking refs are basis refs")
+  val th7 = let
+    val g2 = th6 |> concl |> dest_imp |> fst
+    val l2 = prove(g2,
+                   EVAL_TAC
+                   \\ REWRITE_TAC [semanticPrimitivesTheory.store_v_11,
+                                   APPEND, CONS_11, basis_ffiTheory.basis_refs_eqs]
+                   \\ simp_tac std_ss []
+                   \\ EVAL_TAC)
+    in MP th6 l2 end
+  val th8 = th7 |> DISCH_ALL |> SIMP_RULE bool_ss [GSYM CONJ_ASSOC, AND_IMP_INTRO]
+  val _ = simple_timer t
+  val _ = print ("prove_sem_thm: done\n")
+  in th8 end;
 
 end
